proof/SimMemInjC.v
@@ -397,7 +397,25 @@ Proof.
   esplits; eauto.
   - econs; ss; try apply MWF; eauto.
     + eapply Mem.inject_extends_compose; eauto.
-      admit "ez".
+      econs; eauto.
+      { econs.
+        - ii. inv H0. replace (ofs + 0) with ofs by omega.
+          destruct (eq_block b2 (Mem.nextblock (tgt sm0))); destruct (zle 0 ofs); destruct (zlt ofs (4 * size_arguments sg));
+            try (eapply Mem.perm_unchanged_on; eauto; ss; des_ifs; omega).
+          subst b2. exploit (PERM ofs). omega. i. eapply Mem.perm_cur. eapply Mem.perm_implies; eauto. econs.
+        - ii. inv H0. eapply Z.divide_0_r.
+        - ii. inv H0. replace (ofs + 0) with ofs by omega.
+          destruct (eq_block b2 (Mem.nextblock (tgt sm0))); destruct (zle 0 ofs); destruct (zlt ofs (4 * size_arguments sg));
+            try (exploit Mem.unchanged_on_contents; eauto; ss; des_ifs; try omega; i; rewrite H0; eapply memval_inject_Reflexive).
+          Transparent Mem.alloc. unfold Mem.alloc in ALC. inv ALC. ss.
+          rewrite PMap.gss. rewrite ZMap.gi. eapply memval_inject_undef.
+      }
+      { i. left. assert(Mem.valid_block m1 b).
+        { r. rewrite NB. eapply Mem.perm_valid_block; eauto. }
+        destruct (eq_block b (Mem.nextblock (tgt sm0))) eqn:BEQ; destruct (zle 0 ofs); destruct (zlt ofs (4 * size_arguments sg));
+          try by (eapply Mem.perm_unchanged_on_2; eauto; ss; rewrite BEQ; eauto; try omega).
+        subst b. eapply Mem.perm_cur. eapply Mem.perm_implies. eapply Mem.perm_alloc_2; eauto. econs.
+      }
     + etransitivity; try apply MWF; eauto.
       unfold tgt_private. ss. u. ii; des. esplits; eauto with congruence.
       unfold Mem.valid_block in *. rewrite <- NB in *. eauto with xomega.
